commit

Src/Prover/Main.lean
@@ -12,13 +12,13 @@ theorem not_mem_of_empty {a b} (h : empty a) : b ∉ a :=
 theorem empty_iff {a} : empty a ↔ ∀ b, b ∉ a :=
 iff_intro (λ h _ => not_mem_of_empty h) (λ h h₁ => exi_elim h₁ h)
 
-theorem nonempty_intro {a} b (h : b ∈ a) : nonempty a :=
+theorem nempty_intro {a} b (h : b ∈ a) : nempty a :=
 not_not_intro # exi_intro b h
 
-theorem nonempty_elim {P : Prop} {a} (h₁ : nonempty a) (h₂ : ∀ b, b ∈ a → P) : P :=
+theorem nempty_elim {P : Prop} {a} (h₁ : nempty a) (h₂ : ∀ b, b ∈ a → P) : P :=
 exi_elim (not_not_elim h₁) h₂
 
-theorem nonempty_iff {a} : nonempty a ↔ ∃ b, b ∈ a :=
+theorem nempty_iff {a} : nempty a ↔ ∃ b, b ∈ a :=
 iff_intro not_not_elim not_not_intro
 
 theorem exi_empty : ∃ a, empty a :=
@@ -32,9 +32,9 @@ notation (priority := high) "∅" => emp
 theorem empty_emp : empty ∅ :=
 some_spec exi_empty
 
-theorem exi_nonempty : ∃ a, nonempty a :=
+theorem exi_nempty : ∃ a, nempty a :=
 exi_elim ax_inf # λ a h₁ => exi_elim h₁ # λ b h₂ => exi_intro a #
-nonempty_intro b # and_left # and_right h₂
+nempty_intro b # and_left # and_right h₂
 
 def filter (a : Set) (P : Set → Prop) : Set :=
 some # ax_spec a P
@@ -42,24 +42,24 @@ some # ax_spec a P
 theorem mem_filter {a b} {P : Set → Prop} : b ∈ filter a P ↔ b ∈ a ∧ P b :=
 some_spec (ax_spec a P) b
 
-def fun_to_pred {α β : Type} (f : α → β) (x : α) (y : β) : Prop :=
+def pred_of_fun {α β : Type} (f : α → β) (x : α) (y : β) : Prop :=
 f x = y
 
-theorem fun_to_pred_iff {α β : Type} {f : α → β} {x : α} {y : β} :
-  fun_to_pred f x y ↔ f x = y :=
+theorem pred_of_fun_iff {α β : Type} {f : α → β} {x : α} {y : β} :
+  pred_of_fun f x y ↔ f x = y :=
 iff_refl
 
-theorem exiu_fun_to_pred {α β : Type} {f : α → β} {x : α} :
-  ∃! (y : β), fun_to_pred f x y :=
+theorem exiu_pred_of_fun {α β : Type} {f : α → β} {x : α} :
+  ∃! (y : β), pred_of_fun f x y :=
 exiu_intro (f x) rfl # λ y h => eq_symm h
 
 def image_aux (a : Set) (f : Set → Set) : Set :=
-some # ax_rep a (fun_to_pred f) # λ b h => exiu_fun_to_pred
+some # ax_rep a (pred_of_fun f) # λ b h => exiu_pred_of_fun
 
 theorem mem_image_aux_of {a b : Set} {f : Set → Set}
   (h : ∃ c, c ∈ a ∧ f c = b) : b ∈ image_aux a f :=
 exi_elim h # λ c h₁ => and_elim h₁ # λ h₂ h₃ =>
-exi_elim (some_spec (ax_rep a (fun_to_pred f) (λ b h => exiu_fun_to_pred)) c h₂) #
+exi_elim (some_spec (ax_rep a (pred_of_fun f) (λ b h => exiu_pred_of_fun)) c h₂) #
 λ d h₄ => and_elim h₄ # λ h₅ h₆ =>
 eq_rec' (λ x => x ∈ image_aux a f) (eq_trans (eq_symm h₃) h₆) h₅
 
@@ -73,16 +73,73 @@ iff_intro
 (λ h => mpr mem_filter # and_intro (mem_image_aux_of h) h)
 
 def singleton (a : Set) : Set :=
-image (some exi_nonempty) # λ b => a
+image (some exi_nempty) # λ b => a
 
 theorem mem_singleton {a b} : b ∈ singleton a ↔ b = a :=
 iff_intro
 (λ h => exi_elim (mp mem_image h) # λ c h₁ => eq_symm # and_right h₁)
-(λ h => mpr mem_image # exi_elim (mp nonempty_iff # some_spec exi_nonempty) #
+(λ h => mpr mem_image # exi_elim (mp nempty_iff # some_spec exi_nempty) #
   λ c h₁ => exi_intro c # and_intro h₁ # eq_symm h)
 
 theorem mem_singleton_self {a} : a ∈ singleton a :=
 mpr mem_singleton rfl
 
--- theorem mem_irrefl {a} : a ∉ a :=
--- sorry
+theorem nempty_singleton {a} : nempty (singleton a) :=
+nempty_intro a mem_singleton_self
+
+theorem mem_irrefl {a} : a ∉ a :=
+exi_elim (ax_reg nempty_singleton) # λ b h => and_elim h # λ h₁ h₂ h₃ => h₂ #
+exi_intro a # and_intro (eq_rec' (λ x => a ∈ x) (mp mem_singleton h₁) h₃)
+mem_singleton_self
+
+-- Conditional
+
+theorem exi_ite_val {α : Type} (P : Prop) (x y : α) :
+  ∃ (z : α), (P → z = x) ∧ (¬P → z = y) :=
+prop_rec (λ m => ∃ (z : α), (m → z = x) ∧ (¬m → z = y))
+(exi_intro x # and_intro (λ _ => rfl) (λ h => false_elim # h trivial))
+(exi_intro y # and_intro false_elim (λ _ => rfl))
+
+def ite {α : Type} (P : Prop) (x y : α) : α :=
+some # exi_ite_val P x y
+
+theorem if_pos {α : Type} {P : Prop} {x y : α} (h : P) : ite P x y = x :=
+and_left (some_spec # exi_ite_val P x y) h
+
+theorem if_neg {α : Type} {P : Prop} {x y : α} (h : ¬P) : ite P x y = y :=
+and_right (some_spec # exi_ite_val P x y) h
+
+theorem split_ifs {α : Type} (F : α → Prop) {P : Prop} {x y : α}
+  (h₁ : P → F x) (h₂ : ¬P → F y) : F (ite P x y) :=
+or_elim (@em P)
+(λ h₃ => eq_rec' F (if_pos h₃) # h₁ h₃)
+(λ h₃ => eq_rec' F (if_neg h₃) # h₂ h₃)
+
+-- Unordered pair
+
+def upair (a b : Set) : Set :=
+image (some ax_inf) # λ c => ite (empty c) a b
+
+theorem nempty_image {a} {f : Set → Set} : nempty (image a f) ↔ nempty a :=
+iff_intro
+(λ h => nempty_elim h # λ b h₁ => exi_elim (mp mem_image h₁) #
+  λ c h₂ => nempty_intro c # and_left h₂)
+(λ h => nempty_elim h # λ b h₁ => nempty_intro (f b) # mpr mem_image #
+  exi_intro b # and_intro h₁ rfl)
+
+theorem not_mem_emp {a} : a ∉ ∅ :=
+not_mem_of_empty empty_emp
+
+theorem empty_iff_eq_emp {a} : empty a ↔ a = ∅ :=
+iff_intro
+(λ h => ax_ext # λ b => iff_intro
+  (λ h₁ => false_elim # not_mem_of_empty h h₁) (λ h₁ => false_elim # not_mem_emp h₁))
+(λ h => eq_rec' empty h empty_emp)
+
+theorem empty_elim (P : Set → Prop) {a} (h₁ : empty a) (h₂ : P ∅) : P a :=
+eq_rec' P (mp empty_iff_eq_emp h₁) h₂
+
+theorem nempty_upair {a b : Set} : nempty (upair a b) :=
+mpr nempty_image # nempty_intro ∅ # exi_elim (some_spec ax_inf) # λ c h =>
+eq_rec (λ x => x ∈ some ax_inf) (mp empty_iff_eq_emp # and_left h) #
+and_left # and_right h
